@prefix rdf: <http://www.w3.org/1999/02/22-rdf-syntax-ns#> .
@prefix rdfs: <http://www.w3.org/2000/01/rdf-schema#> .
@prefix owl: <http://www.w3.org/2002/07/owl#> .

<http://rdflib.net/2002/InformationStore>
    a owl:Ontology ;
    rdfs:comment """A document defining a vocabulary used by an InformationStore, a TripleStore
            with support for multiple contexts.""" ;
    rdfs:isDefinedBy <http://rdflib.net/2002/InformationStore> ;
    rdfs:label "InformationStore" .

<http://rdflib.net/2002/InformationStore#Context>
    a rdfs:Class ;
    rdfs:isDefinedBy <http://rdflib.net/2002/InformationStore> ;
    rdfs:label "Context" ;
    rdfs:subClassOf rdfs:Resource .

<http://rdflib.net/2002/InformationStore#UpdateEvent>
    a rdfs:Class ;
    rdfs:isDefinedBy <http://rdflib.net/2002/InformationStore> ;
    rdfs:label "An Event for updating a Context" ;
    rdfs:subClassOf rdfs:Resource .

<http://rdflib.net/2002/InformationStore#error>
    a rdf:Property ;
    rdfs:comment """This property is used to capture information about errors that occured while
            updating the context.""" ;
    rdfs:domain rdfs:UpdateEvent ;
    rdfs:isDefinedBy <http://rdflib.net/2002/InformationStore> ;
    rdfs:label "Error" ;
    rdfs:range rdfs:Literal .

<http://rdflib.net/2002/InformationStore#http_status>
    a rdf:Property ;
    rdfs:comment """This property is used for the http status that was returned when updating the
            context.""" ;
    rdfs:domain rdfs:UpdateEvent ;
    rdfs:isDefinedBy <http://rdflib.net/2002/InformationStore> ;
    rdfs:label "http status" ;
    rdfs:range rdfs:Literal .

<http://rdflib.net/2002/InformationStore#source>
    a rdf:Property ;
    rdfs:domain rdfs:Resource ;
    rdfs:isDefinedBy <http://rdflib.net/2002/InformationStore> ;
    rdfs:label "source" ;
    rdfs:range rdfs:Resource .

<http://rdflib.net/2002/InformationStore#updateEvent>
    a rdf:Property ;
    rdfs:domain rdfs:Context ;
    rdfs:isDefinedBy <http://rdflib.net/2002/InformationStore> ;
    rdfs:label "update event" ;
    rdfs:range rdfs:UpdateEvent .

